src/program_logic/staged_invariant_use_cancel.v
@@ -54,7 +54,8 @@ Proof using later_tokG0.
   iIntros "Hsv".
   iLöb as "IH" forall (e).
   iDestruct "Hsv" as (E2 ? mj_ishare mj_ushare ????? Hsub)
-    "(%Hnval&%Hinvalid&%Heq_mj&%Hle2&%Hinvalid2&Hown&Hownstat&#Hsaved1&#Hsaved2&[Hltok Htoklc]&Hitok&%Hlt2&#Hinv)".
+    "(%Hnval&%Hinvalid&%Heq_mj&%Hle2&%Hinvalid2&Hown&Hownstat&#Hsaved1&#Hsaved2&Hltok&Hitok&%Hlt2&#Hinv)".
+  iDestruct (later_tokN_use with "[$]") as "[Htoklc Hcl]". simpl.
   iEval (rewrite wpc0_unfold).
   rewrite /wpc_pre. iSplit; last first.
   {
@@ -162,11 +163,10 @@ Proof using later_tokG0.
     replace (⊤ ∖ D ∖ E2) with (⊤ ∖ (E2 ∪ D)) by set_solver.
     iDestruct ("Hwp" with "[$] [$] [$]") as "Hwp". iModIntro.
     iSplit; [by iLeft in "Hwp"|iRight in "Hwp"].
-    iIntros (e2 ????). iDestruct ("Hwp" with "[//]") as "Hwp".
-    iApply (physical_step_tr_use with "[$]").
-    iApply (physical_step_wand with "Hwp").
-    iIntros "(Hstate&Hg&H&Hefs&HNC) H⧗ H£".
-    iFrame "Hstate". iModIntro.
+    iIntros (e2 ????).
+    iMod "Hcl" as "_". iApply (physical_step_wand with "(Hwp [//])").
+    iIntros "(Hstate&Hg&H&Hefs&HNC) /= [Htok _]".
+    iFrame "Hstate".
 
     destruct (to_val e2) eqn:Heq_val.
     {
@@ -253,21 +253,7 @@ Proof using later_tokG0.
     }
     iApply "IH".
     iExists _, _, mj_ishare, _, _, _, _, _. iExists _. iFrame "∗".
-    iSplit; first eauto.
-    iFrame "Hsaved1'' Hsaved2''".
-    iSplit; first eauto.
-    iSplit; first eauto.
-    iSplit.
-    { iPureIntro. rewrite /mj_wp. naive_solver. }
-    iSplit; first eauto.
-    iSplit; first eauto.
-    iSplit.
-    { assert (2 ≤ f 2) by (pose proof (f_exp 2); lia).
-      iDestruct (lc_weaken with "H£") as "$"; first done.
-      by iApply (tr_weaken with "H⧗").
-    }
-    iSplit; first eauto.
-    iExact "Hinv".
+    repeat iSplit; try eauto.
   }
 Qed.
 
@@ -280,7 +266,7 @@ Lemma wpc_staged_inv_use_cancel E1 e Φ Φc Qs P :
   ⊢ WPC e @ E1 {{ Φ }} {{ Φc }}.
 Proof using later_tokG0.
   iIntros (Hnval) "(Hstaged&Hwp)".
-  iDestruct "Hstaged" as (E2 ??? γprop γprop') "(Hown&Hownstat&#Hsaved1&#Hsaved2&[Hltok Htoklc]&Hitok&Hinv)".
+  iDestruct "Hstaged" as (E2 ??? γprop γprop') "(Hown&Hownstat&#Hsaved1&#Hsaved2&Hltok&Hitok&Hinv)".
   iDestruct "Hinv" as (mj_wp_init mj_ishare Hlt) "#Hinv".
   rewrite /staged_inv.
   rewrite wpc_eq /wpc_def. iIntros (mj).
@@ -312,7 +298,8 @@ Proof using later_tokG0.
   iDestruct (saved_prop_agree with "Hsaved1 Hsaved1'") as "Hequiv1".
   iDestruct (saved_prop_agree with "Hsaved2 Hsaved2'") as "Hequiv2".
 
-  iApply (lc_fupd2_add_laterN with "Htoklc"). iNext. iNext.
+  iDestruct(later_tokN_use with "[$]") as "[Htoklc Hcl]".
+  iApply (lc_fupd2_add_laterN with "Htoklc"). iNext.
   iDestruct "Hinner" as "[HPs|Hfin]"; last first.
   { (* Impossible, since we have NC token. *)
     iDestruct "Hfin" as "(_&HC&_)". iDestruct (NC_C with "[$] [$]") as %[]. }
@@ -359,11 +346,9 @@ Proof using later_tokG0.
   iDestruct ("Hwp" with "[$] [$] [$]") as "Hwp". iModIntro.
   iSplit; [by iLeft in "Hwp"|iRight in "Hwp"].
   iIntros (e2 σ2 g2 efs Hstep).
-  iDestruct ("Hwp" with "[//]") as "Hwp".
-
-  iApply (physical_step_tr_use with "[$]").
-  iApply (physical_step_wand with "Hwp").
-  iIntros "($&Hg&H&Hefs&HNC) H⧗ H£ !>".
+  
+  iMod "Hcl". simpl. iApply (physical_step_wand with "(Hwp [//])").
+  iIntros "($&Hg&H&Hefs&HNC) [Htok _]".
   destruct (to_val e2) eqn:Heq_val.
   {
     iEval (rewrite wpc0_unfold /wpc_pre) in "H".
@@ -463,27 +448,14 @@ Proof using later_tokG0.
   iAssert (staged_value_inuse_cancel e2 ⊤ ⊤ mj mj_wp mj_ukeep Φ Φc P) with "[-]" as "Hsv".
   {
     iExists _, _, mj_ishare, _, _, _, _, _. iExists _. iFrame "∗".
-    iSplit; first eauto.
-    iFrame "Hsaved1'' Hsaved2''".
-    iSplit; first eauto.
-    iSplit; first eauto.
-    iSplit; first eauto.
-    iSplit.
+    repeat iSplit; eauto.
     { iPureIntro. rewrite /mj_wp.
       etransitivity; first eapply Qp.le_min_l.
       etransitivity; first eapply Qp.le_min_l.
       eapply Qp.le_min_r. }
-    iSplit.
     { iPureIntro. rewrite /mj_wp.
       etransitivity; first eapply Qp.le_min_l.
       eapply Qp.le_min_r. }
-    iSplit.
-    { assert (2 ≤ f 2) by (pose proof (f_exp 2); lia).
-      iDestruct (lc_weaken with "H£") as "$"; first done.
-      by iApply (tr_weaken with "H⧗").
-    }
-    iSplit; first eauto.
-    iExact "Hinv".
   }
   iApply (wpc_staged_inv_inuse_cancel_aux with "[$]").
 Qed.
